- move to_bexpr properties to a new file - fix an obvious bug in br_app_anno

src-lite/bidirectional.v
@@ -1,218 +1,10 @@
-Require Import decl.properties.
-Require Import decl.ln_inf.
 Require Import Program.Tactics.
+
+Require Import decl.properties.
 Require Import bidir.notations.
 Require Import bidir.properties.
 Require Import bidir.elaboration.
-
-Require Import Lia.
-
-Set Printing Parentheses.
-
-Fixpoint to_bexpr (e : expr) : bexpr :=
-  match e with
-  | e_var_f x => be_var_f x
-  | e_var_b x => be_var_b x
-  | e_kind k_star => be_kind bk_star
-  | e_kind k_box => be_kind bk_box
-  | e_num n => be_num n
-  | e_int => be_int
-  | e_bot A => be_anno be_bot (to_bexpr A)
-  | e_app f a => be_app (to_bexpr f) (to_bexpr a)
-  | e_abs  A (b_anno e B) => be_anno (be_abs  (to_bexpr e)) (be_pi  (to_bexpr A) (to_bexpr B))
-  | e_bind A (b_anno e B) => be_anno (be_bind (to_bexpr e)) (be_all (to_bexpr A) (to_bexpr B))
-  | e_pi  A B => be_pi  (to_bexpr A) (to_bexpr B)
-  | e_all A B => be_all (to_bexpr A) (to_bexpr B)
-  | e_castup A e => be_anno (be_castup (to_bexpr e)) (to_bexpr A)
-  | e_castdn e => be_castdn (to_bexpr e)
-  end
-.
-
-Fixpoint to_bcontext (Γ : context) : bcontext :=
-  match Γ with
-  | ctx_nil => bctx_nil
-  | ctx_cons Γ' x A => bctx_cons (to_bcontext Γ') x (to_bexpr A)
-  end
-.
-
-Definition to_bk (k : kind) : bkind :=
-  match k with
-  | k_star => bk_star
-  | k_box => bk_box
-  end
-.
-
-
-Lemma size_expr_lt_size_body : forall n e A,
-    size_body (b_anno e A) < S n -> size_expr e < n /\ size_expr A < n.
-Proof.
-  intros. unfold size_body in H. fold size_expr in H. lia.
-Qed.
-
-
-Ltac eq_swap_open_bexpr_with_to_bexpr IHn x:=
-  match goal with
-  | [ _ : _ |- eq (_ (open_bexpr_wrt_bexpr_rec ?n0 _(to_bexpr ?A))) ?Q ] 
-      => rewrite (IHn A n0 x); auto; lia
-  | [ _ : _ |- eq (_ (open_bexpr_wrt_bexpr_rec ?n0 _ (to_bexpr ?A1)) (open_bexpr_wrt_bexpr_rec ?n1 _ (to_bexpr ?A2))) _ ] 
-      => rewrite (IHn A1 n0 x); try rewrite (IHn A2 n1 x); auto; lia
-  | [ _ : _ |- eq (_ (_ (open_bexpr_wrt_bexpr_rec ?n0 _ (to_bexpr ?A1))) (open_bexpr_wrt_bexpr_rec ?n1 _ (to_bexpr ?A2))) _ ] 
-      => rewrite (IHn A1 n0 x); try rewrite (IHn A2 n1 x); auto; lia
-  end.
-
-
-Lemma open_bexpr_wrt_bexpr_rec_exchanges_to_bexpr : forall n A n0 x,
-    size_expr A < n -> 
-    open_bexpr_wrt_bexpr_rec n0 `' x (to_bexpr A) = to_bexpr (open_expr_wrt_expr_rec n0 ` x A).
-Proof.
-  intro n. induction n.
-  - intros. inversion H.
-  - intro A. induction A; intros; auto; simpl in *;try (eq_swap_open_bexpr_with_to_bexpr IHn x).
-    + destruct (lt_eq_lt_dec n0 n1).
-      * destruct s; auto; lia.
-      * auto.
-    + destruct k; auto.
-    + destruct b. simpl.
-      assert (size_body (b_anno e A0) < S n). { lia. } specialize (size_expr_lt_size_body n e A0 H0). intro.
-      rewrite (IHA n0 x). rewrite (IHn e (S n0) x). rewrite (IHn A0 (S n0) x).
-      auto. all : lia.
-    + destruct b. simpl.
-      assert (size_body (b_anno e A0) < S n). { lia. } specialize (size_expr_lt_size_body n e A0 H0). intro.
-      rewrite (IHA n0 x). rewrite (IHn e (S n0) x). rewrite (IHn A0 (S n0) x).
-      auto. all : lia.
-Qed.
-
-Ltac swap_open_expr_wrt_bexpr_rec_with_to_bexpr :=
-  match goal with 
-  | _ : _ |- lc_bexpr (open_bexpr_wrt_bexpr_rec 1 `' ?x (to_bexpr ?A) ^`' _) => 
-    rewrite (open_bexpr_wrt_bexpr_rec_exchanges_to_bexpr (S (size_expr A)) A 1 x); auto; lia
-  end.
-      
-
-Theorem lc_tobexpr : forall A x,
-    lc_bexpr (to_bexpr (A ^` x))
-  -> lc_bexpr (to_bexpr A ^`' x).
-Proof.
-  intros. dependent induction A; auto.
-  - destruct n.
-    + constructor.
-    + simpl in *. unfold open_bexpr_wrt_bexpr. simpl. auto.
-  - destruct k; constructor.
-  - inversion H. constructor; eauto.
-  - inversion H. constructor; eauto. 
-  - unfold to_bexpr. destruct b.
-    constructor; fold open_bexpr_wrt_bexpr_rec; fold to_bexpr.
-    + inversion H. inversion H2. constructor. intro. swap_open_expr_wrt_bexpr_rec_with_to_bexpr.
-    + inversion H. inversion H3. constructor.
-      * apply IHA. assumption.
-      * intros. swap_open_expr_wrt_bexpr_rec_with_to_bexpr.
-  - inversion H. constructor; fold open_bexpr_wrt_bexpr_rec; fold to_bexpr.
-    + apply IHA1. auto.
-    + intros. specialize (H3 x0). swap_open_expr_wrt_bexpr_rec_with_to_bexpr.
-  - unfold to_bexpr. destruct b. inversion H. constructor; fold open_bexpr_wrt_bexpr_rec; fold to_bexpr.
-    + constructor. intro. inversion H2. swap_open_expr_wrt_bexpr_rec_with_to_bexpr.
-    + constructor; inversion H3. eauto.
-      intro. swap_open_expr_wrt_bexpr_rec_with_to_bexpr.
-  - inversion H. constructor; fold open_bexpr_wrt_bexpr_rec; fold to_bexpr.
-    + apply IHA1. assumption. 
-    + intro. swap_open_expr_wrt_bexpr_rec_with_to_bexpr.
-  - inversion H; constructor.
-    + inversion H2. constructor. apply IHA2. auto.
-    + eauto.
-  - inversion H; constructor; eauto.
-Qed.
-
-Ltac solve_lc_bexpr_with_to_bexpr_and_open := 
-  match goal with 
-  | H : forall x, ?P -> ?Q -> lc_bexpr (to_bexpr x) |- lc_bexpr (to_bexpr ?A ^`' ?x) =>
-        apply lc_tobexpr; eapply H; try (unfold open_expr_wrt_expr; rewrite (size_expr_open_expr_wrt_expr_rec_var A x 0); lia); try auto
-  end.
-
-Scheme Induction for lc_expr Sort Prop
-  with Induction for lc_body Sort Prop.
-
-Theorem to_bexpr_keeps_lc : forall A,lc_expr A -> lc_bexpr (to_bexpr A).
-Proof.
-  intros A.
-  apply lc_expr_ind_dep with
-  (P := fun e (_ : lc_expr e) => lc_bexpr (to_bexpr e))
-  (P0 := fun b  (_ : lc_body b) => match b with (b_anno e A)  => lc_bexpr (to_bexpr e) /\ lc_bexpr (to_bexpr A) end); intros; try (simpl; auto).
-  - destruct k; auto.
-  - destruct b. constructor.
-    + constructor. intro. specialize (H0 x). simpl in H0. inversion H0. apply lc_tobexpr. auto.
-    + constructor. auto. intro. specialize (H0 x). simpl in H0. inversion H0. apply lc_tobexpr. auto.
-  - constructor.
-    + auto. 
-    + intros. specialize (H0 x). apply lc_tobexpr. auto.
-  - destruct b. constructor.
-    + constructor. intro. specialize (H0 x). simpl in H0. inversion H0. apply lc_tobexpr. auto.
-    + constructor.
-      * auto.
-      * intros. specialize (H0 x). simpl in H0. inversion H0. apply lc_tobexpr. auto.
-  - constructor. 
-    + auto.
-    + intros. specialize (H0 x). apply lc_tobexpr. auto.
-Qed. 
-
-
-Theorem to_bcontext_keeps_lc : forall Γ, lc_context Γ -> lc_bcontext (to_bcontext Γ).
-Proof.
-  intros.
-  induction Γ.
-  - auto.
-  - simpl. constructor; inversion H; subst.
-    + apply IHΓ. auto.
-    + eapply to_bexpr_keeps_lc; auto.
-Qed.
-
-
-Theorem to_bcontext_keeps_notin : forall x G, 
-  x `notin` ctx_dom G
-  -> x `notin` bctx_dom (to_bcontext G).
-Proof.
-  intros. induction G.
-  - auto.
-  - simpl in *.
-    eapply notin_add_3.
-    + eapply notin_add_1'. eauto.
-    + eapply notin_add_2. eauto.
-Qed.
-
-Ltac rewrite_to_expr A x := 
-  match goal with 
-  | [ _ : _ |- _ ] 
-  => unfold open_bexpr_wrt_bexpr; rewrite (open_bexpr_wrt_bexpr_rec_exchanges_to_bexpr (S (size_expr A)) A 0 x (le_lt_n_Sm (size_expr A) (size_expr A) (le_n (size_expr A)))); fold open_expr_wrt_expr_rec
- end.
-
- Scheme Induction for expr Sort Prop
-  with Induction for body Sort Prop.
-
-Theorem to_bexpr_keeps_mono_type: forall t,
-  mono_type t -> mono_btype (to_bexpr t).
-Proof.
-  intros. 
-  dependent induction H; try constructor; auto.
-  - destruct k; constructor.
-  - fold to_bexpr. apply to_bexpr_keeps_lc. auto.
-  - simpl. econstructor; auto. intros.
-    specialize (H1 x H2). rewrite_to_expr B x. auto.
-  - constructor. apply to_bexpr_keeps_lc. auto.
-    intros. fold to_bexpr. inversion H0.
-    specialize (H6 x). inversion H6. auto. 
-    apply lc_tobexpr.
-    apply to_bexpr_keeps_lc. auto.
-  - fold to_bexpr.
-    econstructor. intros.
-    rewrite_to_expr e x. apply H2. auto.
-  - constructor. apply to_bexpr_keeps_lc. auto.
-    inversion H0.
-    intro. specialize (H6 x).
-    inversion H6. apply lc_tobexpr. apply to_bexpr_keeps_lc.  
-    auto.
-  - econstructor.
-    intros. fold to_bexpr. rewrite_to_expr e x. apply H2. auto.
-  - apply to_bexpr_keeps_lc. auto.
-Qed.
+Require Import transform_properties.
 
 
 Theorem bidir_complete : forall Γ e1 e2 A
@@ -282,13 +74,13 @@ Proof.
       destruct k2; auto.
     + intros. specialize (H3 x H4). rewrite_to_expr B1 x. rewrite_to_expr B2 x.
       destruct k2; auto.
-  - econstructor; fold to_bexpr.
+  - eapply bs_app with (A:=(to_bexpr (e_pi A0 B))); fold to_bexpr.
     + apply to_bexpr_keeps_mono_type. auto.
-    + eauto.
-    + simpl. replace (to_bexpr (B ^^ t)) with ((to_bexpr) B ^^' (to_bexpr t)).  econstructor.
-    * admit.  (* *** *)
-    * eapply bs_sub. eauto. admit. (* ** *)
-    * admit. (* * *)
+    + auto.
+    + replace (to_bexpr (B ^^ t)) with ((to_bexpr B) ^^' (to_bexpr t)) by admit. econstructor; fold to_bexpr.
+      * intros. admit. (* substitution *)
+      * eapply bs_sub. exact H0.
+        admit. (* type_correctness *)
   - econstructor; fold to_bexpr.
     + eapply bs_bind with (k:=to_bk k) (L:=L); fold to_bexpr.
       * apply bidir_refl_l in H0. destruct k; auto.
@@ -299,8 +91,12 @@ Proof.
         rewrite_to_expr e0 x. rewrite_to_expr e3 x. eauto.
         rewrite_to_expr B1 x. 
         specialize (H2 x H5). apply bidir_refl_l in H2. simpl in H2. auto.
-      * admit. (* * *)
-      * admit. (* * *)
+      * intros. rewrite_to_expr e0 x.
+        specialize (n x H5). rewrite (to_bexpr_keeps_fv (e0 ^` x)) in n.
+        apply n.
+      * intros. rewrite_to_expr e3 x.
+        specialize (n0 x H5). rewrite (to_bexpr_keeps_fv (e3 ^` x)) in n0.
+        apply n0.
     + eapply bs_forall with (k:=to_bk k); fold to_bexpr.
       * destruct k; eauto.
       * destruct k; eauto.
@@ -314,19 +110,21 @@ Proof.
         replace ((to_bcontext G),' x : (to_bexpr A1)) with ((to_bcontext G),' x : (to_bexpr A1),,'bctx_nil) in H3.
         eapply bidir_narrowing with (A:=to_bexpr A2) (k:=to_bk k) in H3.
         auto. destruct k; auto. auto.
-  - simpl. eapply bs_anno with (k:=to_bk k).
-    eapply bs_sub with (A := to_bexpr B) (k:=to_bk k).
+  - simpl. eapply bs_anno with (k:=to_bk k). 
+    eapply bs_castup with (k:=to_bk k) (B:=to_bexpr B).
+    + apply bidir_refl_l in H0. destruct k; auto. 
     + admit. (* *** *)
-    + admit. (* ** *)
+    + eapply bs_sub with (A:=to_bexpr B). auto.
+      admit. (* type_correctness *) 
     + destruct k; auto.
     + destruct k; auto.
-  - eapply bs_castdn with (k:=to_bk k) (A:=to_bexpr A0). 
+  - eapply bs_castdn with (k:=to_bk k) (A:=to_bexpr A0); fold to_bexpr. 
     + destruct k; auto.
     + constructor. 
-      * apply to_bcontext_keeps_lc. admit. (* ** *)
-      * admit. (* * *)
-    + fold to_bexpr. eauto.
-  - eapply bs_forall_l with (t:=to_bexpr t) (k:=to_bk k); fold to_bexpr.
+      * apply to_bcontext_keeps_lc. apply wf_lc. admit. 
+      * admit. (* *** *)
+    + auto.
+   - eapply bs_forall_l with (t:=to_bexpr t) (k:=to_bk k); fold to_bexpr.
     + apply to_bexpr_keeps_mono_type. auto.
     + destruct k; auto.
     + eapply bs_sub with (k:=to_bk k); eauto.
@@ -344,8 +142,7 @@ Proof.
     + destruct k; auto.
     + intros. fold to_bexpr. specialize (H2 x H3). simpl in H2.
       rewrite_to_expr B x. rewrite_to_expr C x. auto. 
-  - admit. (* ** *)
-
+  - admit. (* *** *) 
 (* wf_context *)
   - constructor.
   - simpl. apply bwf_cons with (k:=to_bk k). 
@@ -359,7 +156,7 @@ Theorem bidir_sound : forall Γ' e1' e2' d A' Γ e1 e2 A,
   busub_elab Γ' e1' e2' d A' Γ e1 e2 A → Γ ⊢ e1 <: e2 : A.
 Proof.
   intros.
-  induct ion H.
+  induction H.
   (* pattern Γ', e1, e2', d, A', Γ, e1, e2, A, H.
   eapply busub_ind_dep with 
     (P0 := fun Γ' (_ : ⫦ Γ') => ⊢ Γ). *)
